inverse_then_mod skeleton

code/experimental/P256/p256-c/Hacl_Impl_MM_Exponent.h
@@ -6,21 +6,21 @@
  */
 
 #include "kremlib.h"
-#ifndef __FStar_H
-#define __FStar_H
+#ifndef __Hacl_Impl_MM_Exponent_H
+#define __Hacl_Impl_MM_Exponent_H
 
-
+#include "FStar.h"
 #include "TestLib.h"
 #include "c/Lib_PrintBuffer.h"
 #include "FStar_UInt_8_16_32_64.h"
 
-extern uint64_t FStar_UInt64_eq_mask(uint64_t x0, uint64_t x1);
+void Hacl_Impl_MM_Exponent_cswap(uint64_t bit, uint64_t *p1, uint64_t *p2);
 
-extern uint128_t FStar_UInt128_shift_right(uint128_t x0, uint32_t x1);
+void Hacl_Impl_MM_Exponent_montgomery_ladder_exponent(uint64_t *a);
 
-extern uint64_t FStar_UInt128_uint128_to_uint64(uint128_t x0);
+void Hacl_Impl_MM_Exponent_fromDomainImpl(uint64_t *a, uint64_t *result);
 
-extern uint128_t FStar_UInt128_mul_wide(uint64_t x0, uint64_t x1);
+void Hacl_Impl_MM_Exponent_multPower(uint64_t *a, uint64_t *b, uint64_t *result);
 
-#define __FStar_H_DEFINED
+#define __Hacl_Impl_MM_Exponent_H_DEFINED
 #endif
