code/experimental/P256/Hacl.Impl.MM.Exponent.fst
@@ -1,0 +1,209 @@
+module Hacl.Impl.MM.Exponent
+
+
+open FStar.HyperStack.All
+open FStar.HyperStack
+module ST = FStar.HyperStack.ST
+
+open Lib.IntTypes
+open Lib.Buffer
+
+open FStar.Math.Lemmas
+
+open Hacl.Spec.P256.Lemmas
+open Hacl.Spec.P256.Definitions
+open Hacl.Impl.LowLevel
+open Hacl.Spec.P256.Basic
+open Hacl.Spec.P256.Core
+
+open FStar.Mul
+
+open Hacl.Impl.MontgomeryMultiplication
+open Lib.Loops
+
+noextract
+val fromDomain_: a: nat -> Tot nat
+
+let fromDomain_ a = (a * modp_inv2_prime (pow2 256) prime) % prime
+
+noextract
+val toDomain_: a: nat -> Tot nat
+let toDomain_ a = (a * pow2 256) % prime 
+
+
+assume val lemmaFromDomainToDomain:  a: nat -> Lemma (toDomain_ (fromDomain_ a)  == a)
+
+assume val inDomain_mod_is_not_mod: a: nat ->  Lemma (toDomain_ a == toDomain_ (a % prime))
+
+assume val lemmaFromDomainToDomainModuloPrime: a: nat -> Lemma (a % prime == fromDomain_(toDomain_ a))
+
+
+
+open Hacl.Spec.P256.Ladder
+
+[@ CInline]
+val cswap: bit:uint64{v bit <= 1} -> p:felem -> q:felem
+  -> Stack unit
+    (requires fun h ->
+      live h p /\ live h q /\ (disjoint p q \/ p == q) /\
+           
+      as_nat h (gsub p (size 0) (size 4)) < prime /\ 
+      as_nat h (gsub p (size 4) (size 4)) < prime /\
+      as_nat h (gsub p (size 8) (size 4)) < prime /\
+	     
+      as_nat h (gsub q (size 0) (size 4)) < prime /\  
+      as_nat h (gsub q (size 4) (size 4)) < prime /\
+      as_nat h (gsub q (size 8) (size 4)) < prime
+)
+    (ensures  fun h0 _ h1 ->
+      modifies (loc p |+| loc q) h0 h1 /\
+      (let pBefore = as_seq h0 p in let qBefore = as_seq h0 q in 
+	let pAfter = as_seq h1 p in let qAfter = as_seq h1 q in 
+	let condP0, condP1 = conditional_swap bit pBefore qBefore  in 
+	condP0 == pAfter /\ condP1 == qAfter) /\ 
+
+      (v bit == 1 ==> as_seq h1 p == as_seq h0 q /\ as_seq h1 q == as_seq h0 p) /\
+      (v bit == 0 ==> as_seq h1 p == as_seq h0 p /\ as_seq h1 q == as_seq h0 q))
+
+
+let cswap bit p1 p2 =
+  let h0 = ST.get () in
+  let mask = u64 0 -. bit in
+  let open Lib.Sequence in 
+  [@ inline_let]
+  let inv h1 (i:nat{i <= 4}) =
+    (forall (k:nat{k < i}).
+      if v bit = 1
+      then (as_seq h1 p1).[k] == (as_seq h0 p2).[k] /\ (as_seq h1 p2).[k] == (as_seq h0 p1).[k]
+      else (as_seq h1 p1).[k] == (as_seq h0 p1).[k] /\ (as_seq h1 p2).[k] == (as_seq h0 p2).[k]) /\
+    (forall (k:nat{i <= k /\ k < 12}).
+      (as_seq h1 p1).[k] == (as_seq h0 p1).[k] /\ (as_seq h1 p2).[k] == (as_seq h0 p2).[k]) /\
+    modifies (loc p1 |+| loc p2) h0 h1 in
+ 
+  Lib.Loops.for 0ul 4ul inv
+    (fun i ->
+      let dummy = mask &. (p1.(i) ^. p2.(i)) in
+      p1.(i) <- p1.(i) ^. dummy;
+      p2.(i) <- p2.(i) ^. dummy;
+      lemma_cswap2_step bit ((as_seq h0 p1).[v i]) ((as_seq h0 p2).[v i])
+    );
+  let h1 = ST.get () in
+  Lib.Sequence.eq_intro (as_seq h1 p1) (if v bit = 1 then as_seq h0 p2 else as_seq h0 p1);
+  Lib.Sequence.eq_intro (as_seq h1 p2) (if v bit = 1 then as_seq h0 p1 else as_seq h0 p2)
+
+inline_for_extraction noextract
+val montgomery_ladder_exponent_step0: a: felem -> b: felem -> Stack unit
+  (requires fun h -> True)
+  (ensures fun h0 _ h1 -> True)
+
+let montgomery_ladder_exponent_step0 a b = 
+  montgomery_multiplication_ecdsa_module a b b;
+  montgomery_multiplication_ecdsa_module a a a
+
+
+
+(* this piece of code is taken from Hacl.Curve25519 *)
+inline_for_extraction noextract 
+val scalar_bit:
+  s:lbuffer uint8 (size 32)
+  -> n:size_t{v n < 256}
+  -> Stack uint64
+    (requires fun h0 -> live h0 s)
+    (ensures  fun h0 r h1 -> h0 == h1 (*/\ r == ith_bit (as_seq h0 s) (v n) /\ v r <= 1) *) )
+
+let scalar_bit s n =
+ let h0 = ST.get () in
+  mod_mask_lemma ((Lib.Sequence.index (as_seq h0 s) (v n / 8)) >>. (n %. 8ul)) 1ul;
+  assert_norm (1 = pow2 1 - 1);
+  uintv_extensionality (mod_mask #U8 1ul) (u8 1);
+  to_u64 ((s.(n /. 8ul) >>. (n %. 8ul)) &. u8 1)
+
+inline_for_extraction noextract 
+val montgomery_ladder_exponent_step: a: felem -> b: felem ->scalar: lbuffer uint8 (size 32) ->   i:size_t{v i < 256} ->  Stack unit
+  (requires fun h -> live h a  /\ live h b)
+  (ensures fun h0 _ h1 -> True)
+
+
+let montgomery_ladder_exponent_step a b scalar i = 
+  let bit0 = (size 255) -. i in 
+  let bit = scalar_bit scalar bit0 in 
+  cswap bit a b;
+  montgomery_ladder_exponent_step0 a b;
+  cswap bit a b;
+  
+  ()
+
+inline_for_extraction noextract 
+val _montgomery_ladder_exponent: a: felem ->b: felem ->  scalar: lbuffer uint8 (size 32) -> Stack unit
+  (requires fun h -> True)
+  (ensures fun h0 _ h1 -> True)
+
+
+let _montgomery_ladder_exponent a b scalar = 
+  [@inline_let]
+  let inv h (i: nat {i <= 256}) = 
+    True in 
+
+  for 0ul 256ul inv (fun i -> montgomery_ladder_exponent_step a b scalar i)
+
+inline_for_extraction noextract 
+val upload_zero_montg_form: b: felem -> Stack unit
+  (requires fun h -> True)
+  (ensures fun h0 _ h1 -> True)
+
+let upload_zero_montg_form b = ()
+
+inline_for_extraction noextract 
+val upload_scalar: b: lbuffer uint8 (size 32) -> Stack unit 
+  (requires fun h -> True)
+  (ensures fun h0 _ h1 -> True)
+
+let upload_scalar b = ()
+
+
+val montgomery_ladder_exponent: a: felem -> Stack unit 
+  (requires fun h -> True)
+  (ensures fun h0 _ h1 -> True)
+
+let montgomery_ladder_exponent a = 
+  push_frame(); 
+    let b = create (size 4) (u64 0) in 
+    let scalar = create (size 32) (u8 0) in 
+    upload_zero_montg_form b;
+    upload_scalar scalar;
+
+    _montgomery_ladder_exponent a b scalar;
+  pop_frame()  
+
+inline_for_extraction noextract 
+val upload_one: one: felem -> Stack unit 
+  (requires fun h -> True)
+  (ensures fun h0 _ h1 -> True)
+
+let upload_one one = admit()
+
+
+val fromDomainImpl: a: felem -> result: felem -> Stack unit
+  (requires fun h -> True)
+  (ensures fun h0 _ h1 -> True)
+
+let fromDomainImpl a result = 
+  push_frame();
+    let one = create (size 4) (u64 0) in 
+    upload_one one;
+    montgomery_multiplication_ecdsa_module one a result;
+  pop_frame()   
+
+
+val multPower: a: felem -> b: felem ->  result: felem -> Stack unit 
+  (requires fun h -> True)
+  (ensures fun h0 _ h1 -> True)
+
+
+let multPower a b result = 
+  push_frame();
+    let tempB1 = create (size 4) (u64 0) in 
+  fromDomainImpl a tempB1;
+  montgomery_ladder_exponent tempB1;
+  montgomery_multiplication_ecdsa_module tempB1 b result;
+  pop_frame()
